Imp/Expr/Optimize.lean
@@ -9,6 +9,12 @@ Optimizes an expression by folding constants.
 def optimize : Expr → Expr
   | .const i => .const i
   | .var x => .var x
+  | .unop uop e =>
+    match optimize e with
+    | .const i =>
+      if let some v := uop.apply i then .const v
+      else .unop uop (.const i)
+    | e' => .unop uop e'
   | .op bop e1 e2 =>
     match optimize e1, optimize e2 with
     | .const i, .const i' =>
@@ -22,6 +28,11 @@ Optimization doesn't change the meaning of any expression
 theorem optimize_ok (e : Expr) : e.eval σ = e.optimize.eval σ := by
   induction e <;> simp [optimize]
   case op bop e1 e2 ih1 ih2 =>
+    split <;> simp [eval, *]
+    split
+    · simp [eval, *]
+    · simp [eval]
+  case unop uop e ih =>
     split <;> simp [eval, *]
     split
     · simp [eval, *]
